Extraction/archsem.mli
@@ -59,7 +59,10 @@ module Arm : sig
       | Strict
   end
 
-  val vmProm_model : ?bbm_param:BBM.param -> empty ArchModel.t
+  val vmProm_model :
+    ?bbm_param:BBM.param ->
+    ?deduplicate_final_states:bool ->
+    empty ArchModel.t
 end
 
 module X86 : sig
